start proving security of protocol under active attacker

theories/approxis/examples/wmf_active_attacker_security.v
@@ -2,11 +2,14 @@ From Ltac2 Require Import Ltac2.
 Set Default Proof Mode "Classic".
 From clutch.approxis Require Import map reltac2 approxis option.
 From clutch.approxis.examples Require Import
-  security_aux option symmetric_init wmf_protocol
-  pubkey advantage_laws iterable_expression.
+  security_aux option symmetric_init wmf_protocol linked_list
+  pubkey advantage_laws iterable_expression intptxt_ideal_dec.
 From mathcomp Require Import ssrbool.
 Set Default Proof Using "All".
 Import map.
+
+Ltac try_close_inv :=
+  try (by (iLeft; iFrame; try_close_inv)); try (by (iRight; iFrame; try_close_inv)).
 
 Section logrel.
 
@@ -15,21 +18,23 @@ Section logrel.
   (* security parameter *)
   Variable η : nat.
 
-  Let N := 2^η.
+  Let N := 2^η - 1.
 
   Variable Key Output : nat.
 
   (* ASSUMPTION ON THE ENCRYPTION SCHEME *)
+  Definition lrel_id : lrel Σ := lrel_nat.
 
-  Definition left_lrel (τ : lrel Σ) (v : val) : iProp Σ := ∃ v', (lrel_car τ) v v'.
-  Definition right_lrel (τ : lrel Σ) (v : val) : iProp Σ := ∃ v', (lrel_car τ) v' v.
-
-  Definition lrel_id : lrel Σ := lrel_int_bounded 0 1.
-
-  Definition lrel_input : lrel Σ := lrel_int_bounded 0 N * lrel_int_bounded 0 N.
   Definition lrel_rand : lrel Σ := lrel_int_bounded 0 N.
-  Variable lrel_output : lrel Σ.
+  Definition lrel_msg : lrel Σ := (lrel_id * lrel_rand)%lrel.
+  Variable lrel_cipher : lrel Σ.
   Variable lrel_key : lrel Σ.
+
+  Definition lrel_protocol : lrel Σ :=
+    lrel_rand →
+      (() + (lrel_id * lrel_cipher)) *
+      ((lrel_id * lrel_cipher) → () + lrel_cipher) *
+      (lrel_cipher → () + ()).
 
   Variable senc : list loc → val.
   Variable sdec : list loc → val.
@@ -83,11 +88,11 @@ Section logrel.
   Hypothesis refines_init_scheme_r : refines_init_scheme_r_prop.
 
   Definition refines_sym_keygen_couple_prop := forall K K' E A,
-    (∀ key,
-      (lrel_car lrel_key) key key -∗
+    (∀ key key',
+      (lrel_car lrel_key) key key' -∗
         refines E
           (fill K  (Val key))
-          (fill K' (Val key))
+          (fill K' (Val key'))
           A)
     ⊢ refines E
         (fill K  (keygen #()))
@@ -138,9 +143,9 @@ Section logrel.
 
   Definition refines_senc_lr_l_prop :=
     ∀ (lls rls : list loc) (msg msg' : val) (k k' : val) K K' E A,
-    lrel_key k k' ∗ lrel_input msg msg' ∗ Plr lls rls ⊢
+    lrel_key k k' ∗ lrel_msg msg msg' ∗ Plr lls rls ⊢
       ((∀ (c c' : val),
-        lrel_output c c'
+        lrel_cipher c c'
       -∗ @sym_is_cipher_lr_l lls rls msg c k
       -∗ refines E
           (fill K (Val c))
@@ -153,9 +158,9 @@ Section logrel.
       
   Definition refines_senc_lr_r_prop :=
     ∀ (lls rls : list loc) (msg msg' : val) (k k' : val) K K' E A,
-    lrel_key k k' ∗ lrel_input msg msg' ∗ Plr lls rls ⊢
+    lrel_key k k' ∗ lrel_msg msg msg' ∗ Plr lls rls ⊢
       ((∀ (c c' : val),
-        lrel_output c c'
+        lrel_cipher c c'
       -∗ @sym_is_cipher_lr_r lls rls msg c' k
       -∗ refines E
           (fill K (Val c))
@@ -179,8 +184,1473 @@ Section logrel.
     ) →
     na_invP 𝒩 P
       ⊢ refines top (senc lls)
-      (senc rls) (lrel_key → lrel_input → lrel_output).
+      (senc rls) (lrel_key → lrel_msg → lrel_cipher).
 
   Hypothesis senc_sem_typed : senc_sem_typed_prop.
+
+  Section linked_list_instance.
+    (* all messages encrypted in this protocol are of the form
+      (an identifier, an integer ≤ N) *)
+
+    Definition elem_eq : val :=
+      λ: "x" "y", Fst "x" = Fst "y" `and` Snd "x" = Snd "y".
+      
+    Lemma refines_elem_eq_l : (refines_elem_eq_l_prop elem_eq
+      (λ x, half_lrel lrel_msg x)).
+    Proof with rel_pures_l.
+      rewrite /refines_elem_eq_l_prop.
+      iIntros (x y).
+      iIntros (K e E A).
+      rewrite /elem_eq...
+      iIntros "[[Hcarx | Hcarx] [[Hcary | Hcary] Hrel]]";
+      rewrite /left_lrel/right_lrel/lrel_msg;
+      iDestruct "Hcarx" as (v_tmp x1 x1' x2 x2')
+      "[%eqx [%eqx' [[%lx [%eqx1 %eqx1']] [%lx' [%eqx2 [%eqx2' _]]]]]]";
+      iDestruct "Hcary" as (v_tmp' y1 y1' y2 y2')
+      "[%eqy [%eqy' [[%ly [%eqy1 %eqy1']] [%ly' [%eqy2 [%eqy2' _]]]]]]"; subst;
+      simpl; rel_pures_l;
+      destruct (bool_decide (#lx = #ly));
+      destruct (bool_decide (#lx' = #ly')); rel_apply "Hrel".
+    Qed.
+
+    Lemma refines_elem_eq_r : (refines_elem_eq_r_prop elem_eq
+      (λ x, half_lrel lrel_msg x)).
+    Proof with rel_pures_r.
+      rewrite /refines_elem_eq_l_prop.
+      iIntros (x y).
+      iIntros (K e E A).
+      rewrite /elem_eq...
+      iIntros "[[Hcarx | Hcarx] [[Hcary | Hcary] Hrel]]";
+      rewrite /left_lrel/right_lrel/lrel_msg;
+      iDestruct "Hcarx" as (v_tmp x1 x1' x2 x2')
+      "[%eqx [%eqx' [[%lx [%eqx1 %eqx1']] [%lx' [%eqx2 [%eqx2' _]]]]]]";
+      iDestruct "Hcary" as (v_tmp' y1 y1' y2 y2')
+      "[%eqy [%eqy' [[%ly [%eqy1 %eqy1']] [%ly' [%eqy2 [%eqy2' _]]]]]]"; subst;
+      simpl; rel_pures_r;
+      destruct (bool_decide (#lx = #ly));
+      destruct (bool_decide (#lx' = #ly')); rel_apply "Hrel".
+    Qed.
+
+  End linked_list_instance.
+
+  Variable is_ciphertext : val.
+  (* all messages encrypted in this protocol are of the form
+    (an identifier, an integer ≤ N) *)
+  Definition is_plaintext : val :=
+    λ: "x", #0 ≤ (Fst "x") `and` #0 ≤ (Snd "x") `and` (Snd "x") ≤ #N.
+  Variable is_key : val.
+
+  Lemma refines_is_plaintext_l : refines_is_plaintext_l_prop lrel_msg is_plaintext.
+  Proof with rel_pures_l.
+    rewrite /refines_is_plaintext_l_prop.
+    iIntros (c K e E A)
+      "[%c' [%x1 [%x2 [%x1' [%x2' [%Heqc [%Heqc' Hcompx]]]]]]] Hrel".
+    iDestruct "Hcompx" as
+      "[[%id [%eqx1 %eqx1']] [%msg [%eqx2 [%eqx2' [%Hbound1 %Hbound2]]]]]"; subst.
+    eapply bool_decide_eq_true in Hbound1;
+    eapply bool_decide_eq_true in Hbound2.
+    assert (Hboundid : bool_decide (0 ≤ id)%Z = true).
+    { apply bool_decide_eq_true. lia. }
+    rewrite /is_plaintext...
+    rewrite Hbound1 Hbound2 Hboundid...
+    rel_apply "Hrel".
+    Unshelve.
+    all: apply Z_le_dec.
+  Qed.
+
+  Hypothesis refines_is_ciphertext_l :
+    @refines_is_ciphertext_l_prop _ _ lrel_cipher is_ciphertext.
+  Hypothesis refines_is_ciphertext_r :
+    @refines_is_ciphertext_r_prop _ _ lrel_cipher is_ciphertext.
+  Hypothesis refines_is_plaintext_r :
+    @refines_is_plaintext_r_prop _ _ lrel_msg is_plaintext.
+  Hypothesis refines_is_plaintext_l :
+    @refines_is_plaintext_l_prop _ _ lrel_msg is_plaintext.
+  Hypothesis refines_is_key_l :
+    @refines_is_key_l_prop _ _ lrel_key is_key.
+  Hypothesis refines_is_key_r :
+    @refines_is_key_r_prop _ _ lrel_key is_key.
+
+  Hypothesis sdec_sem_typed : @sdec_sem_typed_prop _ _
+    lrel_msg lrel_cipher lrel_key sdec Plr.
+
+  Definition refines_couple_sdec_prop := ∀ K K' E (A : lrel Σ) k k' c c' lls rls,
+       Plr lls rls
+    -∗ lrel_key k k'
+    -∗ lrel_cipher c c'
+    -∗
+    ((∀ decr decr', lrel_msg decr decr' -∗ Plr lls rls -∗
+      (REL fill K (Val decr) << fill K' (Val decr') @ E : A))
+    -∗ REL fill K (sdec lls k c) << fill K' (sdec rls k' c') @ E : A).
+  
+  Hypothesis refines_couple_sdec : refines_couple_sdec_prop.
+
+  Definition PTXT' : val := PTXT' is_ciphertext is_plaintext elem_eq.
+
+  Definition PTXT'' : val :=
+    λ: "b" "adv" "scheme" "Q_enc_key" "Q_enc" "Q_dec",
+      let: "record_plaintext" := init_linked_list #() in
+      let: "enc_scheme" := get_enc_scheme "scheme" #() in
+      let: "enc" := get_enc "enc_scheme" in
+      let: "dec" := get_dec "enc_scheme" in
+      let: "key" := get_keygen "scheme" #() in
+      let: "enc_key" := λ: "msg", add_list "record_plaintext" "msg";;
+        "enc" "key" "msg" in
+      let: "oracle_enc_key" := q_calls_general_test is_plaintext "Q_enc" "enc_key" in
+      let: "oracle_enc" :=
+        q_calls_general_test
+          (λ: "p", is_key (Fst "p") `and` is_plaintext (Snd "p"))
+          "Q_enc"
+          (λ: "p", "enc" (Fst "p") (Snd "p")) in
+      let: "oracle_enc" := λ: "k" "msg", "oracle_enc" ("k", "msg") in
+      let: "oracle_lr" :=
+        let: "counter" := ref #0 in
+        λ: "c",
+          if: "b" then
+            if: is_ciphertext "c" then
+              let: "decrypted" := "dec" "key" "c" in
+              if: ! "counter" < "Q_dec" then
+                "counter" <- ! "counter" + #1;;
+                let: "decrypted'" := "dec" "key" "c" in
+                if: elem_of_linked_list elem_eq
+                  "record_plaintext" "decrypted'" then
+                  SOME "decrypted"
+                else
+                  NONEV
+              else NONEV
+            else NONEV
+          else
+            if: is_ciphertext "c" then
+              if: ! "counter" < "Q_dec" then
+                "counter" <- ! "counter" + #1;;
+                SOME ("dec" "key" "c")
+              else NONEV
+            else NONEV
+      in
+      let: "b'" := "adv" "oracle_enc_key" "oracle_enc" "oracle_lr" in
+      "b'".
+  
+  Let wmf_once := wmf_once η Key Output.
+
+  Definition a_to_s_adv : val :=
+    λ:  "A" "B" "b" "senc_oracle",
+      let: "run" := ref #true in
+      λ: "r_adv",
+        if: ! "run" then
+          "run" <- #false;;
+          SOME
+            (if: "b" then
+              let: "nonce" := rand #N in
+              let:m "c" := "senc_oracle" ("B", "nonce") in
+              ("A", "c")
+            else
+              let:m "c" := "senc_oracle" ("B", "r_adv") in
+              ("A", "c"))
+        else NONE.
+
+  Definition s_to_b_adv : val :=
+    λ: "A" "B" "b" "senc_oracle" "sdec_oracle_a" "kb",
+      let: "run" := ref #true in
+      λ: "input",
+        if: ! "run" then
+          "run" <- #false;;
+          let:m "nonce" := "sdec_oracle_a" (Snd "input") in
+          let: "sender" := Fst "input" in
+          let: "dest" := Fst "nonce" in
+          let: "nonce" := Snd "nonce" in
+          if: "sender" = "A" `and` "dest" = "B" then
+            "senc_oracle" "kb" ("sender", "nonce")
+          else (**"senc_oracle" "kb" ("sender", "nonce");;*) NONE
+        else NONE.
+
+  Definition wmf_once_adv_ptxt : expr :=
+    let: "B" := init_id #() in  
+    let: "A" := Fst "B" in
+    let: "B" := Snd "B" in
+    λ: "b" "enc_oracle_a" "enc_oracle" "dec_oracle_a",
+      let: "kb" := keygen #() in
+        let: "a_to_s" := a_to_s_adv "A" "B" "b"
+          "enc_oracle_a" in
+        let: "s_to_b" := s_to_b_adv "A" "B" "b"
+          "enc_oracle" "dec_oracle_a" "kb" in
+        let: "b_recv" := b_recv_once "A" "B" "b" "kb" in
+      λ: "r_adv",
+        ("a_to_s" "r_adv",
+         "s_to_b",
+         "b_recv").
+
+  #[local] Instance wmf_msg_inj : Inject val val.
+  Proof. unshelve econstructor.
+    - exact (λ x, x).
+    - intros x y H; done.
+  Defined.
+
+  Lemma wmf_once_true__wmf_adv_ptxt_false (adv : val) :
+      (lrel_protocol → lrel_bool)%lrel adv adv
+    ⊢ REL (adv (init_scheme (wmf_once #true))) <<
+        (PTXT'' #false
+          (λ: "senc_oracle" "senc_oracle_gen" "sdec_oracle",
+            adv (wmf_once_adv_ptxt #true
+              "senc_oracle" "senc_oracle_gen" "sdec_oracle"))
+          sym_scheme
+          #1 #1 #1)
+      : lrel_bool.
+  Proof with rel_pures_l; rel_pures_r.
+    iIntros "#Hreladv".
+    rewrite /init_scheme/wmf_protocol.init_scheme/PTXT''.
+      (* /PTXT'/intptxt_ideal_dec.PTXT''. *)
+    rel_apply refines_init_scheme_l.
+    iIntros (lls) "HP"...
+    rel_apply refines_init_list_r.
+    iIntros (record) "Hrecord"...
+    rel_apply refines_init_scheme_r.
+    iIntros (rls) "HP'"...
+    rewrite /get_enc/get_dec/get_keygen...
+    rewrite /init_id...
+    rel_apply refines_sym_keygen_couple.
+    iIntros (ka ka') "#Hrelka"...
+    rewrite /q_calls_general_test...
+    rel_alloc_r cnt_enc as "Hcntenc".
+    rel_alloc_r cnt_encgen as "Hcntencgen".
+    rel_alloc_r cnt_dec as "Hcntdec"...
+    rewrite /init_id...
+    rel_bind_l _.
+    rel_bind_r (adv _).
+    rel_apply (refines_bind with "[-]").
+    2: {
+      iIntros (v v') "Hrelv"...
+      rel_vals.
+    }
+    rel_apply refines_app; first rel_vals.
+    iClear "Hreladv".
+    rel_apply refines_sym_keygen_couple.
+    iIntros (kb kb') "#Hrelkb"...
+    rewrite /a_to_s_once/a_to_s_adv...
+    rel_alloc_l run1 as "Hrun1";
+    rel_alloc_r run1' as "Hrun1'"...
+    rewrite /s_to_b_once/s_to_b_adv/get_enc...
+    rel_alloc_l run2 as "Hrun2";
+    rel_alloc_r run2' as "Hrun2'"...
+    rewrite /b_recv_once...
+    rel_alloc_l run3 as "Hrun3";
+    rel_alloc_r run3' as "Hrun3'"...
+    set (P := (
+          Plr lls rls ∗ (
+            run1  ↦  #false
+          ∗ run1' ↦ₛ #false
+          ∗ (∃ (nonce : nat),
+                linked_slist wmf_msg_inj record [(#1, #nonce)%V]
+              ∗ True)
+          ∗ cnt_enc ↦ₛ #1
+          ∗ ( run2  ↦  #false
+            ∗ run2' ↦ₛ #false
+            ∗ cnt_dec ↦ₛ #1
+            ∗ (cnt_encgen ↦ₛ #1 ∨ cnt_encgen ↦ₛ #0)
+            ∗ ( run3  ↦  #false
+              ∗ run3' ↦ₛ #false ∨
+                run3  ↦  #true
+              ∗ run3' ↦ₛ #true)
+            ∨ run2  ↦  #true
+            ∗ run2' ↦ₛ #true
+            ∗ cnt_dec ↦ₛ #0
+            ∗ cnt_encgen ↦ₛ #0
+            ∗ ( run3  ↦  #false
+              ∗ run3' ↦ₛ #false ∨
+                run3  ↦  #true
+              ∗ run3' ↦ₛ #true))
+          ∨ run1  ↦  #true
+          ∗ run1' ↦ₛ #true
+          ∗ linked_slist wmf_msg_inj record []
+          ∗ cnt_enc ↦ₛ #0
+          ∗ ( run2  ↦  #false
+            ∗ run2' ↦ₛ #false
+            ∗ cnt_dec ↦ₛ #1
+            ∗ (cnt_encgen ↦ₛ #1 ∨ cnt_encgen ↦ₛ #0)
+            ∗ ( run3  ↦  #false
+              ∗ run3' ↦ₛ #false ∨
+                run3  ↦  #true
+              ∗ run3' ↦ₛ #true)
+            ∨ run2  ↦  #true
+            ∗ run2' ↦ₛ #true
+            ∗ cnt_dec ↦ₛ #0
+            ∗ cnt_encgen ↦ₛ #0
+            ∗ ( run3  ↦  #false
+              ∗ run3' ↦ₛ #false ∨
+                run3  ↦  #true
+              ∗ run3' ↦ₛ #true))
+        ))%I).
+    rel_apply (refines_na_alloc P (nroot.@"wmf_once__wmf_adv_ptxt_true".@"global")).
+    iSplitL.
+    { iSplitL "HP HP'";
+      first iApply (P0lr_Plr with "HP HP'").
+      repeat (iRight; iFrame). }
+    iIntros "#Inv". rewrite /lrel_protocol.
+    rel_arrow_val.
+    iIntros (v1 v2) "[%r_adv [%eq1 [%eq2 %Hradvbound]]]"; subst...
+    repeat rel_apply refines_pair.
+    - rel_apply refines_na_inv; iSplit; first iAssumption.
+      iIntros "[
+        [HP
+          [[Hrun1 [Hrun1' [Hlst [Hcnt H]]]]|[Hrun1 [Hrun1' [Hlst [Hcnt H]]]]]]
+        Hclose]"; rel_load_l; rel_load_r...
+      + rel_apply refines_na_close. iFrame. iSplitL; first (iLeft; iFrame).
+        rel_vals.
+      + rel_store_l; rel_store_r...
+        rel_apply refines_couple_UU; first done.
+        iModIntro; iIntros (nonce Hnoncebound)...
+        rel_apply refines_is_plaintext_r.
+        {
+          iExists _.
+          iExists _, _, _, _.
+          repeat iSplit.
+          * iPureIntro; done.
+          * iPureIntro; done.
+          * iExists 1. iPureIntro; split; done.
+          * iExists nonce. iPureIntro; repeat split; lia.
+        }
+        rel_load_r... rel_load_r; rel_store_r...
+        replace ((#1, #nonce)%V) with (inject (#1, #nonce)%V) by done.
+        rel_apply (refines_add_list_r with "[-Hlst]").
+        2: { iAssumption. }
+        iIntros "Hlst"...
+        rel_apply refines_na_close. iFrame.
+        iSplitL.
+        {
+          iLeft. iFrame.
+        }
+        rel_bind_l (senc _ _ _);
+        rel_bind_r (senc _ _ _).
+        rel_apply refines_bind.
+        { repeat rel_apply refines_app; first (iApply senc_sem_typed; last iAssumption).
+          - eexists. apply bi.equiv_entails. split; iIntros "H"; first last.
+            + iDestruct "H" as "[HP H]"; iFrame. iAssumption.
+            + iDestruct "H" as "[HP H]"; iFrame.
+          - rel_vals.
+          - rel_vals; first iExists 1; last iExists _; iPureIntro; repeat split; lia.
+        }
+        iIntros (v v') "#Hrel"...
+        rel_vals; first iExists 0; done.
+    - rel_arrow_val.
+      iIntros (input1 input2) "[%id_ [%id_' [%c [%c'
+        [%Hinputeq1 [%Hinputeq2 [[%id [%eqid1 %eqid2]] #Hrelcipher]]]]]]]"; subst...
+      rel_apply refines_na_inv; iSplit; first iAssumption.
+      iIntros "[
+        [HP
+          [[Hrun1 [Hrun1' [Hlst [Hcnt_enc [
+            [Hrun2 [Hrun2' [Hcnt_dec H]]]|
+            [Hrun2 [Hrun2' [Hcnt_dec H]]]
+            ]]]]] |
+           [Hrun1 [Hrun1' [Hlst [Hcnt_enc [
+            [Hrun2 [Hrun2' [Hcnt_dec H]]]|
+            [Hrun2 [Hrun2' [Hcnt_dec H]]]
+            ]]]]]]]
+        Hclose]"; rel_load_l; rel_load_r; rel_pures_l; rel_pures_r;
+      try by (
+        rel_apply refines_na_close; iFrame; iSplitL;
+          try (by try (iLeft; iFrame; iLeft; iFrame); rel_vals);
+          try (by try (iLeft; iFrame; iRight; iFrame); rel_vals);
+          try (by try (iRight; iFrame; iLeft; iFrame); rel_vals "ka");
+          try (by try (iRight; iFrame; iRight; iFrame); rel_vals))...
+      + rel_store_l; rel_store_r...
+        rel_apply (refines_is_ciphertext_r with "[Hrelcipher]")...
+        { iExists c. iAssumption. }
+        rel_load_r; rel_load_r; rel_store_r...
+        rel_apply (refines_couple_sdec with "HP").
+        1, 2: iAssumption.
+        iIntros (decrypted1 decrypted2) "[%iddest [%iddest' [%crecv [%crecv'
+        [%Hinputeq1 [%Hinputeq2 [[%id_dest
+          [%eqiddest1 %eqiddest2]] [%r [%eqr1 [%eqr2 %Hrbound]]]]]]]]]] HP"; subst...
+        destruct (bool_decide (#id = #0)) eqn:eqid;
+        destruct (bool_decide (#id_dest = #1)) eqn:eqiddest...
+        2, 3, 4:
+          rel_apply refines_na_close;
+          iFrame; iSplitL; first
+          (
+            iFrame; iLeft; iFrame; iLeft; iFrame;
+            iDestruct "H" as "[Hcnt H]"; iSplitR "H";
+            last iAssumption;
+            iRight; done
+          );
+          rel_vals.
+        rel_apply refines_is_plaintext_r...
+        { iExists (#id, #r)%V. iExists _, _, _, _.
+          repeat iSplit. 1, 2: iPureIntro; done.
+          - iExists id. done.
+          - iExists r. iPureIntro; repeat split; lia. }
+        rel_apply refines_is_key_r...
+        {
+          iExists kb. iAssumption.
+        }
+        iDestruct "H" as "[Hcntencgen H]".
+        rel_load_r... rel_load_r; rel_store_r...
+        rel_apply refines_na_close.
+        iFrame; iSplitL.
+        { iFrame. iLeft. iFrame. iLeft; iFrame. }
+        rel_apply refines_injr.
+        repeat rel_apply refines_app.
+        * rel_apply senc_sem_typed; last iAssumption.
+            eexists. apply bi.equiv_entails.
+            split; iIntros "H".
+            -- iDestruct "H" as "[HP H]"; iFrame. iAssumption.
+            -- iDestruct "H" as "[H HP]"; iFrame.
+        * rel_vals.
+        * rel_vals.
+          -- iExists id. done.
+          -- iExists r. done.
+      + rel_store_l; rel_store_r...
+        rel_apply (refines_is_ciphertext_r with "[Hrelcipher]")...
+        { iExists c. iAssumption. }
+        rel_load_r; rel_load_r; rel_store_r...
+        rel_apply (refines_couple_sdec with "HP").
+        1, 2: iAssumption.
+        iIntros (decrypted1 decrypted2) "[%iddest [%iddest' [%crecv [%crecv'
+        [%Hinputeq1 [%Hinputeq2 [[%id_dest
+          [%eqiddest1 %eqiddest2]] [%r [%eqr1 [%eqr2 %Hrbound]]]]]]]]]] HP"; subst...
+        destruct (bool_decide (#id = #0)) eqn:eqid;
+        destruct (bool_decide (#id_dest = #1)) eqn:eqiddest...
+        2, 3, 4:
+          rel_apply refines_na_close;
+          iFrame; iSplitL; first
+          (
+            iFrame; iRight; iFrame; iLeft; iFrame;
+            iDestruct "H" as "[Hcnt H]"; iSplitR "H";
+            last iAssumption;
+            iRight; done
+          );
+          rel_vals.
+        rel_apply refines_is_plaintext_r...
+        { iExists (#id, #r)%V. iExists _, _, _, _.
+          repeat iSplit. 1, 2: iPureIntro; done.
+          - iExists id. done.
+          - iExists r. iPureIntro; repeat split; lia. }
+        rel_apply refines_is_key_r...
+        {
+          iExists kb. iAssumption.
+        }
+        iDestruct "H" as "[Hcntencgen H]".
+        rel_load_r... rel_load_r; rel_store_r...
+        rel_apply refines_na_close.
+        iFrame; iSplitL.
+        { iFrame. iRight. iFrame. iLeft; iFrame. }
+        rel_apply refines_injr.
+        repeat rel_apply refines_app.
+        * rel_apply senc_sem_typed; last iAssumption.
+            eexists. apply bi.equiv_entails.
+            split; iIntros "H".
+            -- iDestruct "H" as "[HP H]"; iFrame. iAssumption.
+            -- iDestruct "H" as "[H HP]"; iFrame.
+        * rel_vals.
+        * rel_vals.
+          -- iExists id. done.
+          -- iExists r. done.
+    - rel_arrow_val.
+      iIntros (input1 input2) "#Hrelcipher"; subst...
+      rel_apply refines_na_inv; iSplit; first iAssumption.
+      iIntros "[
+        [HP
+          [[Hrun1 [Hrun1' [Hlst [Hcnt_enc [
+            [Hrun2 [Hrun2' [Hcnt_dec [Hcntgen [[Hcnt3 Hcnt3'] | [Hcnt3 Hcnt3']] ]]]]|
+            [Hrun2 [Hrun2' [Hcnt_dec [Hcntgen [[Hcnt3 Hcnt3'] | [Hcnt3 Hcnt3']] ]]]]
+            ]]]]] |
+           [Hrun1 [Hrun1' [Hlst [Hcnt_enc [
+            [Hrun2 [Hrun2' [Hcnt_dec [Hcntgen [[Hcnt3 Hcnt3'] | [Hcnt3 Hcnt3']] ]]]]|
+            [Hrun2 [Hrun2' [Hcnt_dec [Hcntgen [[Hcnt3 Hcnt3'] | [Hcnt3 Hcnt3']] ]]]]
+            ]]]]]]]
+        Hclose]";
+      rel_load_l; rel_load_r;
+      try (rel_store_l; rel_store_r); rel_pures_l; rel_pures_r.
+      all: rel_apply refines_na_close; iFrame; iSplitL; first (
+        try (by try (iLeft; iFrame; iLeft; iFrame; iLeft; iFrame));
+        try (by try (iLeft; iFrame; iLeft; iFrame; iRight; iFrame));
+        try (by try (iLeft; iFrame; iRight; iFrame; iLeft; iFrame));
+        try (by try (iLeft; iFrame; iRight; iFrame; iRight; iFrame));
+        try (by try (iRight; iFrame; iLeft; iFrame; iLeft; iFrame));
+        try (by try (iRight; iFrame; iLeft; iFrame; iRight; iFrame));
+        try (by try (iRight; iFrame; iRight; iFrame; iLeft; iFrame));
+        try (by try (iRight; iFrame; iRight; iFrame; iRight; iFrame))
+      ).
+      all: rel_vals.
+  Qed.
+
+  (* We use the PTXT assumption to establish some kind
+    of private channel between a and s *)
+  Definition a_to_s_private_channel : val :=
+    λ:  "A" "B" "b" "channel" "senc" "ka",
+      let: "run" := ref #true in
+      λ: "r_adv",
+        if: ! "run" then
+          "run" <- #false;;
+          SOME
+            (if: "b" then
+              let: "nonce" := rand #N in
+              "channel" <- SOME ("B", "nonce");;
+              let: "c" := "senc" "ka" ("B", "nonce") in
+              ("A", "c")
+            else
+              "channel" <- SOME ("B", "r_adv");;
+              let:m "c" := "senc" "ka" ("B", "r_adv") in
+              ("A", "c"))
+        else NONE.
+
+  Definition s_to_b_private_channel : val :=
+    λ: "A" "B" "b" "channel" "senc" "sdec" "ka" "kb",
+      let: "run" := ref #true in
+      λ: "input",
+        if: ! "run" then
+          "run" <- #false;;
+          let: "decr" := "sdec" "ka" (Snd "input") in
+          let:m "ptxt" := ! "channel" in
+          if: elem_eq "decr" "ptxt" then
+            let: "sender" := Fst "input" in
+            let: "dest" := Fst "ptxt" in
+            let: "nonce" := Snd "ptxt" in
+            if: "sender" = "A" `and` "dest" = "B" then
+              SOME ("senc" "kb" ("sender", "nonce"))
+            else NONE
+          else NONE
+        else NONE.
+
+  Definition wmf_once_private_channel : expr :=
+    let: "B" := init_id #() in  
+    let: "A" := Fst "B" in
+    let: "B" := Snd "B" in
+    let: "a_s__channel" := ref NONE in 
+    λ: "b" "enc_scheme",
+      let: "ka" := keygen #() in
+      let: "kb" := keygen #() in
+        let: "a_to_s" := a_to_s_private_channel "A" "B" "b" "a_s__channel"
+          (get_enc "enc_scheme") "ka" in
+        let: "s_to_b" := s_to_b_private_channel "A" "B" "b" "a_s__channel"
+          (get_enc "enc_scheme") (get_dec "enc_scheme") "ka" "kb" in
+        let: "b_recv" := b_recv_once "A" "B" "b" "kb" in
+      λ: "r_adv",
+        ("a_to_s" "r_adv",
+         "s_to_b",
+         "b_recv").
+
+  Definition refines_sdec_lr_l_prop :=
+    ∀ (lls rls : list loc) (c c' : val) (k k' : val) K K' E A,
+    lrel_key k k' ∗ lrel_cipher c c' ∗ Plr lls rls ⊢
+      ((∀ (m m' : val),
+        lrel_msg m m'
+      -∗ @sym_is_cipher_lr_l lls rls m c k
+      -∗ refines E
+          (fill K (Val m))
+          (fill K' (Val m'))
+          A)
+    -∗ refines E
+        (fill K  (sdec lls k  c ))
+        (fill K' (sdec rls k' c'))
+        A).
+
+  Definition refines_sdec_lr_r_prop :=
+    ∀ (lls rls : list loc) (c c' : val) (k k' : val) K K' E A,
+    lrel_key k k' ∗ lrel_cipher c c' ∗ Plr lls rls ⊢
+      ((∀ (m m' : val),
+        lrel_msg m m'
+      -∗ @sym_is_cipher_lr_r lls rls m c k
+      -∗ refines E
+          (fill K (Val m))
+          (fill K' (Val m'))
+          A)
+    -∗ refines E
+        (fill K  (sdec lls k  c ))
+        (fill K' (sdec rls k' c'))
+        A).
+
+  Hypothesis refines_sdec_lr_l : refines_sdec_lr_l_prop.
+  Hypothesis refines_sdec_lr_r : refines_sdec_lr_r_prop.
+
+  Lemma wmf_adv_ptxt_false__wmf_private_channel_true (adv : val) :
+      (lrel_protocol → lrel_bool)%lrel adv adv
+    ⊢ REL
+        (PTXT'' #true
+          (λ: "senc_oracle" "senc_oracle_gen" "sdec_oracle",
+            adv (wmf_once_adv_ptxt #true
+              "senc_oracle" "senc_oracle_gen" "sdec_oracle"))
+          sym_scheme
+          #1 #1 #1) <<
+        (adv (init_scheme (wmf_once_private_channel #true)))
+      : lrel_bool.
+  Proof with rel_pures_l; rel_pures_r.
+    iIntros "#Hadv".
+    rewrite /PTXT''/init_scheme/wmf_protocol.init_scheme...
+    rel_apply refines_init_list_l.
+    Unshelve.
+    2: exact val.
+    2: apply _.
+    iIntros (l_record) "Hrecordlst"...
+    rel_apply refines_init_scheme_l;
+    iIntros (lls) "HP";
+    rel_apply refines_init_scheme_r;
+    iIntros (rls) "HP'"...
+    rewrite /get_enc/get_dec/get_keygen...
+    rewrite /init_id...
+    rel_alloc_r channel as "Hchannel"...
+    rel_apply refines_sym_keygen_couple.
+    iIntros (ka ka') "#Hrelka"...
+    rewrite /q_calls_general_test...
+    rel_alloc_l cnt_enc as "Hcntenc".
+    rel_alloc_l cnt_encgen as "Hcntencgen".
+    rel_alloc_l cnt_dec as "Hcntdec"...
+    rewrite /init_id...
+    rel_bind_l (adv _).
+    rel_bind_r (adv _).
+    rel_apply (refines_bind with "[-]").
+    2: {
+      iIntros (v v') "Hrelv"...
+      rel_vals.
+    }
+    rel_apply (refines_app with "[]"); first (rel_vals; iAssumption).
+    rel_apply refines_sym_keygen_couple.
+    iIntros (kb kb') "#Hrelkb"...
+    rewrite /a_to_s_adv/a_to_s_private_channel...
+    rel_alloc_l run1 as "Hrun1";
+    rel_alloc_r run1' as "Hrun1'"...
+    rewrite /s_to_b_adv/s_to_b_private_channel.
+    rel_alloc_l run2 as "Hrun2";
+    rel_alloc_r run2' as "Hrun2'"...
+    rewrite /b_recv_once...
+    rel_alloc_l run3 as "Hrun3";
+    rel_alloc_r run3' as "Hrun3'"...
+    set (P := (
+          Plr lls rls ∗ (
+            run1  ↦  #false
+          ∗ run1' ↦ₛ #false
+          ∗ (∃ (nonce : nat),
+                linked_list wmf_msg_inj l_record [(#1, #nonce)%V]
+              ∗ channel ↦ₛ SOMEV (#1, #nonce)%V
+              ∗ ⌜nonce ≤ N⌝)
+          ∗ cnt_enc ↦ #1
+          ∗ ( run2  ↦  #false
+            ∗ run2' ↦ₛ #false
+            ∗ cnt_dec ↦ #1
+            ∗ (cnt_encgen ↦ #1 ∨ cnt_encgen ↦ #0)
+            ∗ ( run3  ↦  #false
+              ∗ run3' ↦ₛ #false ∨
+                run3  ↦  #true
+              ∗ run3' ↦ₛ #true)
+            ∨ run2  ↦  #true
+            ∗ run2' ↦ₛ #true
+            ∗ cnt_dec ↦ #0
+            ∗ cnt_encgen ↦ #0
+            ∗ ( run3  ↦  #false
+              ∗ run3' ↦ₛ #false ∨
+                run3  ↦  #true
+              ∗ run3' ↦ₛ #true))
+          ∨ run1  ↦  #true
+          ∗ run1' ↦ₛ #true
+          ∗ (linked_list wmf_msg_inj l_record []
+          ∗ channel ↦ₛ NONEV)
+          ∗ cnt_enc ↦ #0
+          ∗ ( run2  ↦  #false
+            ∗ run2' ↦ₛ #false
+            ∗ cnt_dec ↦ #1
+            ∗ (cnt_encgen ↦ #1 ∨ cnt_encgen ↦ #0)
+            ∗ ( run3  ↦  #false
+              ∗ run3' ↦ₛ #false ∨
+                run3  ↦  #true
+              ∗ run3' ↦ₛ #true)
+            ∨ run2  ↦  #true
+            ∗ run2' ↦ₛ #true
+            ∗ cnt_dec ↦ #0
+            ∗ cnt_encgen ↦ #0
+            ∗ ( run3  ↦  #false
+              ∗ run3' ↦ₛ #false ∨
+                run3  ↦  #true
+              ∗ run3' ↦ₛ #true))
+        ))%I).
+    rel_apply (refines_na_alloc P (nroot.@"wmf_once__wmf_adv_ptxt_true".@"global")).
+    iSplitL.
+    { iSplitL "HP HP'";
+      first iApply (P0lr_Plr with "HP HP'").
+      repeat (iRight; iFrame). }
+    iIntros "#Inv".
+    rel_arrow_val.
+    iIntros (radv1 radv2) "[%r_adv [%eq1 [%eq2 %Hradvbound]]]"; subst...
+    repeat rel_apply refines_pair.
+    - rel_apply refines_na_inv. iSplit; first iAssumption.
+      iIntros "[
+        [HP
+          [[Hrun1 [Hrun1' [Hlst [Hcnt H]]]]|[Hrun1 [Hrun1' [[Hlst Hchannel] [Hcnt H]]]]]]
+        Hclose]"; rel_load_l; rel_load_r...
+      + rel_apply refines_na_close. iFrame. iSplitL.
+        { iLeft. iFrame. }
+        rel_vals.
+      + rel_store_l; rel_store_r...
+        rel_apply refines_couple_UU; first done.
+        iModIntro; iIntros (nonce Hnoncebound)...
+        rel_apply refines_is_plaintext_l.
+        { iExists (#1, #nonce)%V. iExists _, _, _, _.
+          repeat iSplit. 1, 2: iPureIntro; done.
+          all: iExists _; iPureIntro; repeat split; try lia.
+          all: rewrite -(Z2Nat.id 1); done. }
+        rel_load_l...
+        rel_load_l; rel_store_l...
+        replace (#1, #nonce)%V with (inject (#1, #nonce)%V) by done.
+        rel_apply (refines_add_list_l with "[-Hlst]"); last iAssumption.
+        iIntros "Hlst"...
+        rel_store_r...
+        rel_apply refines_na_close.
+        iFrame. iSplitL.
+        { iLeft. iFrame. done. }
+        rel_bind_l (senc _ _ _).
+        rel_bind_r (senc _ _ _).
+        rel_apply refines_bind.
+        2: {
+          iIntros (c1 c2) "#Hrelc"...
+          rel_vals; last iAssumption.
+          iExists 0; done.
+        }
+        repeat rel_apply refines_app.
+        * rel_apply senc_sem_typed; last iAssumption.
+          eexists. apply bi.equiv_entails; split; iIntros "H".
+          -- iDestruct "H" as "[H HP]". iFrame. iAssumption.
+          -- iDestruct "H" as "[H HP]". iFrame.
+        * rel_vals.
+        * rel_vals; iExists _; iPureIntro; repeat split;
+          try rewrite -(Z2Nat.id 1); try lia; done.
+    - rel_arrow_val.
+      iIntros (input1 input2) "[%id_ [%id_' [%c [%c'
+        [%Hinputeq1 [%Hinputeq2 [[%id [%eqid1 %eqid2]] #Hrelcipher]]]]]]]"; subst...
+      rel_apply refines_na_inv; iSplitL; first iAssumption.
+      iIntros "[
+        [HP
+          [[Hrun1 [Hrun1' [Hlst [Hcnt H]]]]|[Hrun1 [Hrun1' [[Hlst Hchannel] [Hcnt H]]]]]]
+        Hclose]";
+      iDestruct "H" as "[[Hrun2 [Hrun2' [Hcntdec [Hcntencgen H]]]] |
+        [Hrun2 [Hrun2' [Hcntdec [Hcntencgen H]]]] ]"; rel_load_l; rel_load_r...
+      1, 3: (rel_apply refines_na_close; iFrame;
+        iSplitL;
+        first try  (iFrame; iLeft; iFrame; iLeft; iFrame);
+        first try  (iFrame; iRight; iFrame; iLeft; iFrame);
+        rel_vals).
+      + rel_store_l; rel_store_r...
+        rel_apply refines_is_ciphertext_l...
+        { iExists c'; done. }
+        rel_apply (refines_sdec_lr_l with "[HP]").
+        {
+          iSplit; first iAssumption.
+          iSplit; first iAssumption.
+          iAssumption.
+        }
+        iIntros (decrypted1 decrypted2) "[%iddest [%iddest' [%crecv [%crecv'
+        [%Hinputeq1 [%Hinputeq2 [[%id_dest
+          [%eqiddest1 %eqiddest2]] [%r [%eqr1 [%eqr2 %Hrbound]]]]]]]]]]
+          Hiscipher"; subst...
+        rel_load_l...
+        rel_load_l... rel_store_l...
+        iDestruct "Hlst" as (nonce) "[Hl_list [Hchannel %Hnoncebound]]".
+        rel_load_r...
+        rel_apply refines_elem_eq_r.
+        iSplitR; last iSplitR.
+        { iLeft. iExists (#id_dest, #r)%V. iExists _, _, _, _.
+          repeat iSplit.
+          1, 2: iPureIntro; done.
+          - iExists id_dest. done.
+          - iExists r. done. }
+        { iLeft. iExists (#1, #nonce)%V. iExists _, _, _, _.
+          repeat iSplit.
+          1, 2: iPureIntro; done.
+          - iExists 1. done.
+          - iExists nonce. iPureIntro; repeat split; lia. }
+        rel_apply "Hiscipher".
+        iIntros "HP"...
+        unshelve rel_apply (refines_elem_of_l lrel_msg with "
+          [Hrun1 Hrun1' Hrun2 Hrun2' Hchannel
+           Hcnt Hcntdec Hcntencgen H Hclose HP]
+          [Hl_list]
+          []"); try iAssumption.
+        1: exact lrel_cipher.
+        1: exact lrel_key.
+        1: exact is_ciphertext.
+        1: exact is_plaintext.
+        1: apply refines_is_ciphertext_r.
+        1: apply refines_is_ciphertext_l.
+        1: apply refines_is_plaintext_r.
+        1: apply refines_is_plaintext_l.
+        3: apply refines_elem_eq_l.
+        3: apply refines_elem_eq_r.
+        1, 2: shelve.
+        2: {
+          iSplit.
+          - simpl. iSplit; last done.
+            iLeft. iExists (#1, #nonce)%V.
+            iExists _, _, _, _. repeat iSplit.
+            1, 2: iPureIntro; done.
+            + iExists 1. iPureIntro. split;
+              f_equal.
+            + iExists nonce. iPureIntro; repeat split; lia. 
+          - simpl.
+            iLeft. iExists (#id_dest, #r)%V.
+            iExists _, _, _, _. repeat iSplit.
+            1, 2: iPureIntro; done.
+            + iExists id_dest. iPureIntro. split;
+              f_equal.
+            + iExists r. iPureIntro; repeat split; lia. 
+        }
+        iIntros (b) "Hlst %eq".
+        rewrite elem_of_list_singleton in eq.
+        destruct (bool_decide (#id_dest = #1)) eqn:Hdecid;
+        destruct (bool_decide (#r = #nonce)) eqn:Hdecr;
+        try apply bool_decide_eq_true in Hdecid as eqid;
+        try apply bool_decide_eq_true in Hdecr as eqr;
+        try apply bool_decide_eq_false in Hdecid as eqid;
+        try apply bool_decide_eq_false in Hdecr as eqr;
+        rel_pures_l; rel_pures_r;
+        try ( destruct b; first
+          ( destruct eq as [eq' _];
+            unshelve epose proof (eq' _) as eq;
+            try done;
+            injection eq;
+            intros eqr' eqid';
+            exfalso; apply eqr; f_equal;
+            rewrite eqr'; done );
+          rel_pures_l; rel_pures_r;
+          rel_apply refines_na_close; iFrame;
+          iSplitL; last rel_vals;
+          iFrame; iLeft; iFrame;
+          iSplitR; first (iPureIntro; lia);
+          iLeft; iFrame ).
+        2: {
+          destruct b...
+          { destruct eq as [eq' _];
+            unshelve epose proof (eq' _) as eq; first done.
+            injection eq;
+            intros eqr' eqid';
+            exfalso; apply eqid; f_equal;
+            rewrite eqid'; done. }
+          rel_apply refines_na_close; iFrame;
+          iSplitL; last rel_vals;
+          iFrame; iLeft; iFrame;
+          iSplitR; first (iPureIntro; lia).
+          iLeft. iFrame. }
+        destruct eq as [_ eqb'].
+        unshelve epose proof (eqb' _) as eqb.
+        { rewrite eqid. rewrite eqr. done. }
+        subst...
+        rewrite eqid...
+        destruct (bool_decide (#id = #0)) eqn:eqid0...
+        2: {
+          rel_apply refines_na_close. iFrame.
+          iSplitL.
+          {
+            iFrame. iLeft. iFrame.
+            iSplitR; first (iPureIntro; lia).
+            iLeft; iFrame.
+          }
+          rel_vals.
+        }
+        rel_apply refines_is_plaintext_l...
+        { iExists (#id, #r)%V. iExists _, _, _, _.
+          repeat iSplit.
+          1, 2 : iPureIntro; done.
+          - iExists id. done.
+          - iExists r. done. }
+        rel_apply refines_is_key_l.
+        { iExists kb'. iAssumption. }
+        rel_load_l...
+        rel_load_l; rel_store_l...
+        rel_apply refines_na_close; iFrame.
+        iSplitL.
+        {
+          iFrame. iLeft. iFrame.
+          iSplitR; first done.
+          iLeft. iFrame.
+        }
+        rewrite eqr.
+        rel_apply refines_injr.
+        repeat rel_apply refines_app.
+        * rel_apply senc_sem_typed; last iAssumption.
+          eexists. apply bi.equiv_entails; split; iIntros "[H1 H2]".
+          -- iFrame. iAssumption.
+          -- iFrame.
+        * rel_vals.
+        * rel_vals.
+          -- iExists id. done.
+          -- iExists nonce. iPureIntro; repeat split; lia.
+        Unshelve.
+        {
+          clear.
+          iIntros (x y) "[[%x' Hx] | [%x' Hx]] [[%y' Hy]|[%y' Hy]]";
+          iDestruct "Hx" as "[%id1v [%id1v' [%m1 [%m1'
+            [%Heq1 [%Heq2 [[%id1
+            [%eqid1 %eqid2]] [%r1 [%eqr1 [%eqr2 %Hr1bound]]]]]]]]]]"; subst;
+          iDestruct "Hy" as "[%id [%id' [%m [%m'
+            [%Heq1 [%Heq2 [[%id2
+            [%eqid1 %eqid2]] [%r2 [%eqr1 [%eqr2 %Hr2bound]]]]]]]]]]"; subst;
+          iPureIntro; constructor; constructor.
+        }
+        {
+          clear.
+          iIntros (x y) "H";
+          iDestruct "H" as "[%id1v [%id1v' [%m1 [%m1'
+            [%Heq1 [%Heq2 [[%id1
+            [%eqid1 %eqid2]] [%r1 [%eqr1 [%eqr2 %Hr1bound]]]]]]]]]]"; subst;
+          done.
+        }
+      + rel_store_l; rel_store_r...
+        rel_apply refines_is_ciphertext_l...
+        { iExists c'; done. }
+        rel_apply (refines_sdec_lr_l with "[HP]").
+        {
+          iSplit; first iAssumption.
+          iSplit; first iAssumption.
+          iAssumption.
+        }
+        iIntros (decrypted1 decrypted2) "[%iddest [%iddest' [%crecv [%crecv'
+        [%Hinputeq1 [%Hinputeq2 [[%id_dest
+          [%eqiddest1 %eqiddest2]] [%r [%eqr1 [%eqr2 %Hrbound]]]]]]]]]]
+          Hiscipher"; subst...
+        rel_load_l...
+        rel_load_l... rel_store_l...
+        rel_load_r...
+        rel_apply "Hiscipher".
+        iIntros "HP"...
+        rel_apply (refines_elem_of_l lrel_msg with "
+          [Hrun1 Hrun1' Hrun2 Hrun2' Hchannel
+           Hcnt Hcntdec Hcntencgen H Hclose HP]
+          [Hlst]
+          []").
+        2: iAssumption.
+        2: {
+          iSplit; first done.
+          simpl.
+          iLeft. iExists (#id_dest, #r)%V.
+          iExists _, _, _, _. repeat iSplit.
+          1, 2: iPureIntro; done.
+          + iExists id_dest. iPureIntro. split;
+            f_equal.
+          + iExists r. iPureIntro; repeat split; lia. 
+        }
+        Unshelve.
+        2: exact lrel_cipher.
+        2: exact lrel_key.
+        2: exact is_ciphertext.
+        2: exact is_plaintext.
+        2: apply refines_is_ciphertext_r.
+        2: apply refines_is_ciphertext_l.
+        2: apply refines_is_plaintext_r.
+        2: apply refines_is_plaintext_l.
+        4: apply refines_elem_eq_l.
+        4: apply refines_elem_eq_r.
+        2, 3: shelve.
+        iIntros (b) "Hlst %eq".
+        destruct b...
+        {
+          exfalso.
+          destruct eq as [eq _].
+          unshelve epose proof (eq _) as eq'; first done.
+          apply elem_of_nil in eq'. assumption.
+        }
+        rel_apply refines_na_close; iFrame.
+        iSplitL.
+        {
+          iFrame. iRight. iFrame.
+          iLeft. iFrame.
+        }
+        rel_vals.
+        Unshelve.
+        {
+          clear.
+          iIntros (x y) "[[%x' Hx] | [%x' Hx]] [[%y' Hy]|[%y' Hy]]";
+          iDestruct "Hx" as "[%id1v [%id1v' [%m1 [%m1'
+            [%Heq1 [%Heq2 [[%id1
+            [%eqid1 %eqid2]] [%r1 [%eqr1 [%eqr2 %Hr1bound]]]]]]]]]]"; subst;
+          iDestruct "Hy" as "[%id [%id' [%m [%m'
+            [%Heq1 [%Heq2 [[%id2
+            [%eqid1 %eqid2]] [%r2 [%eqr1 [%eqr2 %Hr2bound]]]]]]]]]]"; subst;
+          iPureIntro; constructor; constructor.
+        }
+        {
+          clear.
+          iIntros (x y) "H";
+          iDestruct "H" as "[%id1v [%id1v' [%m1 [%m1'
+            [%Heq1 [%Heq2 [[%id1
+            [%eqid1 %eqid2]] [%r1 [%eqr1 [%eqr2 %Hr1bound]]]]]]]]]]"; subst;
+          done.
+        }
+    - rel_arrow_val. iIntros (v1 v2) "#Hrelinput"...
+      rel_apply refines_na_inv. iSplit; first iAssumption.
+      iIntros "[
+        [HP
+          [[Hrun1 [Hrun1' [Hlst [Hcnt H]]]]|[Hrun1 [Hrun1' [[Hlst Hchannel] [Hcnt H]]]]]]
+        Hclose]";
+      iDestruct "H" as "[[Hrun2 [Hrun2' [Hcntdec [Hcntencgen H]]]] |
+        [Hrun2 [Hrun2' [Hcntdec [Hcntencgen H]]]] ]";
+        iDestruct "H" as "[[Hrun3 Hrun3'] | [Hrun3 Hrun3']]";
+        rel_load_l; try rel_store_l;
+        rel_load_r; try rel_store_r;
+        rel_apply refines_na_close; iFrame;
+        iSplitL;
+        try_close_inv;
+        rel_pures_l; rel_pures_r;
+        rel_vals.
+  Qed.
+
+  Definition a_to_s_plain_and_cipher_channel : val :=
+    λ:  "A" "B" "b" "plain_channel" "cipher_channel" "senc" "ka",
+      let: "run" := ref #true in
+      λ: "r_adv",
+        if: ! "run" then
+          "run" <- #false;;
+          SOME
+            (if: "b" then
+              let: "nonce" := rand #N in
+              "plain_channel" <- SOME ("B", "nonce");;
+              let: "c" := "senc" "ka" ("B", "nonce") in
+              "cipher_channel" <- SOME "c";;
+              ("A", "c")
+            else
+              "plain_channel" <- SOME ("B", "r_adv");;
+              let:m "c" := "senc" "ka" ("B", "r_adv") in
+              "cipher_channel" <- SOME "c";;
+              ("A", "c"))
+        else NONE.
+
+  Definition s_to_b_plain_and_cipher_channel : val :=
+    λ: "A" "B" "b" "plain_channel" "cipher_channel" "senc" "sdec" "ka" "kb",
+      let: "run" := ref #true in
+      λ: "input",
+        if: ! "run" then
+          "run" <- #false;;
+          let: "cipher" := Snd "input" in
+          let:m "cipher_rec" := ! "cipher_channel" in
+          let:m "plain_rec" := ! "plain_channel" in
+          let: "decr" := if: "cipher" = "cipher_rec" then
+              "plain_rec"
+            else
+              "sdec" "ka" (Snd "input")
+            in
+          if: elem_eq "decr" "plain_rec" then
+            let: "sender" := Fst "input" in
+            let: "dest" := Fst "plain_rec" in
+            let: "nonce" := Snd "plain_rec" in
+            if: "sender" = "A" `and` "dest" = "B" then
+              SOME ("senc" "kb" ("sender", "nonce"))
+            else NONE
+          else NONE
+        else NONE.
+
+  Definition wmf_once_plain_cipher_channel : expr :=
+    let: "B" := init_id #() in  
+    let: "A" := Fst "B" in
+    let: "B" := Snd "B" in
+    let: "a_s__channel_plain" := ref NONE in 
+    let: "a_s__channel_cipher" := ref NONE in 
+    λ: "b" "enc_scheme",
+      let: "ka" := keygen #() in
+      let: "kb" := keygen #() in
+        let: "a_to_s" := a_to_s_plain_and_cipher_channel "A" "B" "b"
+          "a_s__channel_plain" "a_s__channel_cipher"
+          (get_enc "enc_scheme") "ka" in
+        let: "s_to_b" := s_to_b_plain_and_cipher_channel "A" "B" "b"
+          "a_s__channel_plain" "a_s__channel_cipher"
+          (get_enc "enc_scheme") (get_dec "enc_scheme") "ka" "kb" in
+        let: "b_recv" := b_recv_once "A" "B" "b" "kb" in
+      λ: "r_adv",
+        ("a_to_s" "r_adv",
+         "s_to_b",
+         "b_recv").
+
+  Hypothesis cipher_comparable : ∀ x y,
+    half_lrel lrel_cipher x ∗ half_lrel lrel_cipher y ⊢ ⌜vals_compare_safe x y⌝.
+  
+  Hypothesis lrel_cipher_eq : ∀ x y, lrel_cipher x y ⊢ ⌜x = y⌝.
+
+  Lemma refines_senc_lr_l2 :
+    ∀ (lls rls : list loc) (msg msg' : val) (k k' : val) K K' E A,
+    lrel_key k k' ∗ lrel_msg msg msg' ∗ Plr lls rls ⊢
+      ((∀ (c c' : val),
+        lrel_cipher c c'
+      -∗ (@sym_is_cipher_lr_l lls rls msg c k ∧ Plr lls rls)
+      -∗ refines E
+          (fill K (Val c))
+          (fill K' (Val c'))
+          A)
+    -∗ refines E
+        (fill K  (senc lls k  msg ))
+        (fill K' (senc rls k' msg'))
+        A).
+  Admitted.
+
+  Lemma refines_sdec_l :
+    ∀ (lls rls : list loc) (c : val) (k k' : val) K e' E A,
+    lrel_key k k' ∗ half_lrel lrel_cipher c ∗ Plr lls rls ⊢
+      ((∀ (msg : val),
+        half_lrel lrel_msg msg
+      -∗ Plr lls rls
+      -∗ refines E
+          (fill K (Val c))
+          e'
+          A)
+    -∗ refines E
+        (fill K  (sdec lls k  c))
+        e'
+        A).
+  Admitted.
+
+  Lemma wmf_private_channel_true__wmf_pctxt_channel_true (adv : val) :
+    ⊢ REL
+        (init_scheme (wmf_once_private_channel #true)) <<
+        (init_scheme (wmf_once_plain_cipher_channel #true))
+      : lrel_protocol.
+  Proof with rel_pures_l; rel_pures_r.
+    rewrite /init_scheme/wmf_protocol.init_scheme...
+    rel_apply refines_init_scheme_l;
+    iIntros (lls) "HP";
+    rel_apply refines_init_scheme_r;
+    iIntros (rls) "HP'"...
+    rewrite /get_enc/get_dec/get_keygen...
+    rewrite /init_id...
+    rel_alloc_l ptxtchannel as "Hptxtchannel"...
+    rel_alloc_r ptxtchannel' as "Hptxtchannel'"...
+    rel_alloc_r ctxtchannel' as "Hctxtchannel'"...
+    rel_apply refines_sym_keygen_couple.
+    iIntros (ka ka') "#Hrelka"...
+    rel_apply refines_sym_keygen_couple.
+    iIntros (kb kb') "#Hrelkb"...
+    rewrite /a_to_s_plain_and_cipher_channel/a_to_s_private_channel...
+    rel_alloc_l run1 as "Hrun1";
+    rel_alloc_r run1' as "Hrun1'"...
+    rewrite /s_to_b_plain_and_cipher_channel/s_to_b_private_channel.
+    rel_alloc_l run2 as "Hrun2";
+    rel_alloc_r run2' as "Hrun2'"...
+    rewrite /b_recv_once...
+    rel_alloc_l run3 as "Hrun3";
+    rel_alloc_r run3' as "Hrun3'"...
+    set (P := (
+          (
+            (run1  ↦  #false
+          ∗ run1' ↦ₛ #false
+          ∗ ∃ (nonce : nat) (c c' : val),
+              ( ptxtchannel ↦ SOMEV (#1, #nonce)
+              ∗ ptxtchannel' ↦ₛ SOMEV (#1, #nonce)
+              ∗ (lrel_cipher c c' ∗ ctxtchannel' ↦ₛ SOMEV c')
+              ∗ ⌜nonce ≤ N⌝
+              ∗ ( run2  ↦  #false
+                ∗ run2' ↦ₛ #false
+                ∗ Plr lls rls
+                ∗ ( run3  ↦  #false
+                  ∗ run3' ↦ₛ #false ∨
+                    run3  ↦  #true
+                  ∗ run3' ↦ₛ #true)
+                ∨ run2  ↦  #true
+                ∗ run2' ↦ₛ #true
+                ∗ (@sym_is_cipher_lr_l lls rls (#1, #nonce)%V c ka ∧ Plr lls rls)
+                ∗ ( run3  ↦  #false
+                  ∗ run3' ↦ₛ #false ∨
+                    run3  ↦  #true
+                  ∗ run3' ↦ₛ #true))))
+          ∨ (run1  ↦  #true
+          ∗ run1' ↦ₛ #true
+          ∗ Plr lls rls
+          ∗ ptxtchannel ↦ NONEV
+          ∗ ptxtchannel' ↦ₛ NONEV
+          ∗ ctxtchannel' ↦ₛ NONEV
+          ∗ ( run2  ↦  #false
+            ∗ run2' ↦ₛ #false
+            ∗ ( run3  ↦  #false
+              ∗ run3' ↦ₛ #false ∨
+                run3  ↦  #true
+              ∗ run3' ↦ₛ #true)
+            ∨ run2  ↦  #true
+            ∗ run2' ↦ₛ #true
+            ∗ ( run3  ↦  #false
+              ∗ run3' ↦ₛ #false ∨
+                run3  ↦  #true
+              ∗ run3' ↦ₛ #true)))
+        ))%I).
+    rel_apply (refines_na_alloc P (nroot.@"wmf_channel__both_channel_true")).
+    iPoseProof (P0lr_Plr with "HP HP'") as "HP".
+    iSplitL.
+    { iFrame. try_close_inv. }
+    iIntros "#Inv".
+    rel_arrow_val.
+    iIntros (v1 v2) "[%r [%eq1 [%eq2 %Hrbound]]]"; subst...
+    rel_apply refines_pair; first rel_apply refines_pair.
+    - rel_apply refines_na_inv; iSplit; first iAssumption.
+      iIntros "[
+        [
+          [Hrun1 [Hrun1' H]] |
+          [Hrun1 [Hrun1' [HP [Hpchan [Hpchan' [Hcchan' H]]]]]]
+        ] Hclose]".
+      + rel_load_l; rel_load_r...
+        rel_apply refines_na_close. iFrame.
+        iSplitL.
+        { try_close_inv. }
+        rel_vals.
+      + rel_load_l; rel_load_r...
+        rel_store_l; rel_store_r...
+        rel_apply refines_couple_UU; first done.
+        iIntros (nonce) "%Hnoncebound"; iModIntro...
+        rel_store_l.
+        rel_store_r...
+        rel_apply (refines_senc_lr_l2 with "[HP]").
+        {
+          iFrame. iSplitL; first iAssumption.
+          iExists _, _, _, _. repeat iSplit.
+          1, 2: done.
+          - iExists 1. done.
+          - iExists nonce. iPureIntro; repeat split; lia.
+        }
+        iIntros (c c') "#Hrelcipher Hcipher"...
+        rel_store_r...
+        rel_apply refines_na_close.
+        iFrame. iSplitL.
+        {
+          rewrite /P. iLeft. iFrame.
+          iExists c.
+          iSplitR.
+          { iAssumption. }
+          iSplitR; first (iPureIntro; lia).
+          iDestruct "H" as "[[Hrun2 [Hrun2' H]] | [Hrun2 [Hrun2' H]]]".
+          - iLeft. iPoseProof (bi.and_elim_r with "Hcipher") as "Hcipher". iFrame.
+          - iRight. iFrame.
+        }
+        rel_vals; last iAssumption.
+        iExists 0. done.
+    - rel_arrow_val.
+      iIntros (input1 input2) "[%id_ [%id_' [%c [%c'
+        [%Hinputeq1 [%Hinputeq2 [[%id [%eqid1 %eqid2]] #Hrelcipher]]]]]]]"; subst...
+      rel_apply refines_na_inv. iSplitL; first iAssumption.
+      iIntros "[
+        [
+          [Hrun1 [Hrun1'
+            [%nonce [%c_rec [%c_rec'
+              [
+                Hpchan [Hpchan' [[#Hrelc Hcchan]
+                  [>%Hnoncebound [[Hrun2 [Hrun2' H]] | [Hrun2 [Hrun2' H]]]]
+                ]]
+              ]
+            ]]]
+          ]] |
+          [Hrun1 [Hrun1' [HP [Hpchan [Hpchan' [Hcchan'
+            [[Hrun2 [Hrun2' H]] | [Hrun2 [Hrun2' H]]]
+          ]]]]]]
+        ] Hclose]".
+      + rel_load_l; rel_load_r...
+        rel_apply refines_na_close.
+        iFrame. iSplitL. { iFrame. iLeft.
+          iFrame. iExists c_rec.
+          iSplitR; first iAssumption.
+          iSplitR; first (iPureIntro; lia).
+          iLeft. iFrame. }
+        rel_vals.
+      + rel_load_l; rel_load_r...
+        rel_store_l; rel_store_r...
+        rel_load_r...
+        rel_load_r...
+        iAssert (half_lrel lrel_cipher c') as "Hcipherc'". { iRight. iExists c. done. }
+        iAssert (half_lrel lrel_cipher c_rec') as "Hciphercrec'". { iRight; iExists c_rec. done. }
+        iPoseProof (cipher_comparable with "[Hcipherc' Hciphercrec']") as "%Hcomparable".
+        { iSplit; first iApply "Hcipherc'". iApply "Hciphercrec'". }
+        rel_pure_r. clear Hcomparable.
+        destruct (bool_decide (c' = c_rec')) eqn:eqc...
+        * iDestruct "H" as "[Hcipher H]".
+          apply bool_decide_eq_true in eqc.
+          iPoseProof (lrel_cipher_eq with "Hrelcipher") as "%eqcc'"; subst.
+          iPoseProof (lrel_cipher_eq with "Hrelc") as "%eqcrec'"; subst.
+          rel_apply "Hcipher".
+          iIntros "HP"...
+          rel_load_l... 
+          rel_apply refines_elem_eq_l.
+          iSplitR; last iSplitR.
+          { iLeft. iExists (#1, #nonce)%V. iExists _, _ , _, _.
+            repeat iSplit.
+            1, 2: done.
+            - iExists 1. done.
+            - iExists nonce. iPureIntro; repeat split; lia. }
+          { iLeft. iExists (#1, #nonce)%V. iExists _, _ , _, _.
+            repeat iSplit.
+            1, 2: done.
+            - iExists 1. done.
+            - iExists nonce. iPureIntro; repeat split; lia. }
+          rel_apply refines_elem_eq_r.
+          iSplitR; last iSplitR.
+          { iLeft. iExists (#1, #nonce)%V. iExists _, _ , _, _.
+            repeat iSplit.
+            1, 2: done.
+            - iExists 1. done.
+            - iExists nonce. iPureIntro; repeat split; lia. }
+          { iLeft. iExists (#1, #nonce)%V. iExists _, _ , _, _.
+            repeat iSplit.
+            1, 2: done.
+            - iExists 1. done.
+            - iExists nonce. iPureIntro; repeat split; lia. }
+          destruct (bool_decide (#nonce = #nonce)) eqn:eqnonce...
+          2: { exfalso. clear -eqnonce. apply bool_decide_eq_false in eqnonce.
+            apply eqnonce. reflexivity. }
+          destruct (bool_decide (#id = #0)) eqn:eqid...
+          -- rel_apply (refines_senc_lr_l2 with "[HP]").
+            { iFrame. iSplit; first iAssumption.
+              iExists _, _, _, _.
+              repeat iSplit.
+              1, 2: done.
+              { iExists id. done. }
+              iExists nonce. iPureIntro; repeat split; lia.
+            }
+            iIntros (newc newc') "#Hrelnewc HP".
+            iPoseProof (bi.and_elim_r with "HP") as "HP".
+            rel_apply refines_na_close. iFrame.
+            iSplitL.
+            {
+              iFrame. iLeft.
+              iFrame. iExists _.
+              iSplitR.
+              - iApply "Hrelcipher".
+              - iSplitR; first (iPureIntro; lia).
+                iLeft. iFrame.
+            }
+            rel_pures_l; rel_pures_r.
+            rel_vals.
+          -- rel_apply refines_na_close. iFrame.
+            iSplitL.
+            {
+              iFrame. iLeft.
+              iFrame. iExists _.
+              iSplitR.
+              - iApply "Hrelcipher".
+              - iSplitR; first (iPureIntro; lia).
+                iLeft. iFrame.
+            }
+            rel_vals.
+        * iDestruct "H" as "[Hcipher H]".
+          rel_apply (refines_couple_sdec with "[Hcipher]").
+          { iPoseProof (bi.and_elim_r with "Hcipher") as "Hcipher".
+            iApply "Hcipher". }
+          { iAssumption. }
+          { iAssumption. }
+          iIntros (decr decr') "#Hreldecr HP"...
+          rel_load_l...
+          rel_apply refines_elem_eq_l.
+          iSplitR.
+          { iLeft. iExists decr'. iAssumption. }
+          iSplitR.
+          { iLeft. iExists (#1, #nonce)%V.
+            iExists _, _, _, _. repeat iSplit.
+            1, 2: done.
+            1: iExists 1; done.
+            iExists nonce; iPureIntro; repeat split; lia. }
+          rel_apply refines_elem_eq_r.
+          iSplitR.
+          { iRight. iExists decr. iAssumption. }
+          iSplitR...
+          { iLeft. iExists (#1, #nonce)%V.
+            iExists _, _, _, _. repeat iSplit.
+            1, 2: done.
+            1: iExists 1; done.
+            iExists nonce; iPureIntro; repeat split; lia. }
+          simpl.
+          iDestruct "Hreldecr" as "[%id_decr1 [%id_decr2 [%c_decr [%c_decr'
+            [%Hinputeq1 [%Hinputeq2 [[%id_decr [%eqid1 %eqid2]] #Hreldecr]]]]]]]"; subst...
+          simpl.
+          iDestruct "Hreldecr" as "[%r_decr [%eqr1 [%eqr2 %Hr_decrbound]]]"; subst...
+          destruct (bool_decide (#id_decr = #1)) eqn:eqid_decr;
+          destruct (bool_decide (#r_decr = #nonce)) eqn:eqr_decr; simpl;
+          try rewrite eqr_decr...
+          2, 3, 4: 
+            rel_apply refines_na_close; iFrame; iSplitL; last rel_vals;
+            iLeft; iFrame; iExists c_rec;
+            iSplitR; first iAssumption; iSplitR; first (iPureIntro; lia);
+            iLeft; iFrame.
+          destruct (bool_decide (#id = #0)) eqn:eqid...
+          -- rel_apply (refines_senc_lr_l2 with "[HP]").
+            { iFrame. iSplit; first iAssumption.
+              iExists _, _, _, _.
+              repeat iSplit.
+              1, 2: done.
+              { iExists id. done. }
+              iExists nonce. iPureIntro; repeat split; lia.
+            }
+            iIntros (newc newc') "#Hrelnewc HP".
+            iPoseProof (bi.and_elim_r with "HP") as "HP".
+            rel_apply refines_na_close. iFrame.
+            iSplitL.
+            {
+              iFrame. iLeft.
+              iFrame. iExists _.
+              iSplitR.
+              - iApply "Hrelc".
+              - iSplitR; first (iPureIntro; lia).
+                iLeft. iFrame.
+            }
+            rel_pures_l; rel_pures_r.
+            rel_vals.
+          -- rel_apply refines_na_close. iFrame.
+            iSplitL.
+            {
+              iFrame. iLeft.
+              iFrame. iExists _.
+              iSplitR.
+              - iApply "Hrelc".
+              - iSplitR; first (iPureIntro; lia).
+                iLeft. iFrame.
+            }
+            rel_vals.
+      + rel_load_l; rel_load_r...
+        rel_apply refines_na_close.
+        iFrame. iSplitL. { iFrame. iRight.
+          iFrame.
+          iLeft. iFrame. }
+        rel_vals.
+      + rel_load_l; rel_load_r...
+        rel_store_l; rel_store_r...
+        rel_load_r...
+        rel_apply (refines_sdec_l with "[HP]").
+        { iSplitR; last iSplitR; try iAssumption.
+          iLeft. iExists c'. iAssumption. }
+        iIntros (msg) "_ HP"...
+        rel_load_l...
+        rel_apply refines_na_close. iFrame. iSplitL.
+        {
+          iFrame. iRight.
+          iFrame. iLeft. iFrame.
+        }
+        rel_vals.
+    - rel_arrow_val.
+      iIntros (v1 v2) "Hrelcipher"...
+      rel_apply refines_na_inv. iSplitL; first iAssumption.
+      iIntros "[
+        [
+          [Hrun1 [Hrun1'
+            [%nonce [%c_rec [%c_rec'
+              [
+                Hpchan [Hpchan' [[#Hrelc Hcchan]
+                  [>%Hnoncebound [[Hrun2 [Hrun2' H]] | [Hrun2 [Hrun2' H]]]]
+                ]]
+              ]
+            ]]]
+          ]] |
+          [Hrun1 [Hrun1' [HP [Hpchan [Hpchan' [Hcchan'
+            [[Hrun2 [Hrun2' H]] | [Hrun2 [Hrun2' H]]]
+          ]]]]]]
+        ] Hclose]".
+      + iDestruct "H" as "[HP [[Hrun3 Hrun3'] | [Hrun3 Hrun3']]]";
+        rel_load_l; rel_load_r; last (rel_store_l; rel_store_r)...
+        all: rel_apply refines_na_close; iFrame; iSplitL; last rel_vals.
+        all: iFrame; iLeft; iFrame; iExists c_rec;
+          iSplitR; first iAssumption; iSplitR; first (iPureIntro; lia).
+        all: iLeft; iFrame; iLeft; iFrame.
+      + iDestruct "H" as "[HP [[Hrun3 Hrun3'] | [Hrun3 Hrun3']]]";
+        rel_load_l; rel_load_r; last (rel_store_l; rel_store_r)...
+        all: rel_apply refines_na_close; iFrame; iSplitL; last rel_vals.
+        all: iFrame; iLeft; iFrame; iExists c_rec;
+          iSplitR; first iAssumption; iSplitR; first (iPureIntro; lia).
+        all: iRight; iFrame; iLeft; iFrame.
+      + iDestruct "H" as "[[Hrun3 Hrun3'] | [Hrun3 Hrun3']]";
+        rel_load_l; rel_load_r; last (rel_store_l; rel_store_r)...
+        all: rel_apply refines_na_close; iFrame; iSplitL; last rel_vals.
+        all: iFrame; iRight; iFrame.
+        all: iLeft; iFrame; iLeft; iFrame.
+      + iDestruct "H" as "[[Hrun3 Hrun3'] | [Hrun3 Hrun3']]";
+        rel_load_l; rel_load_r; last (rel_store_l; rel_store_r)...
+        all: rel_apply refines_na_close; iFrame; iSplitL; last rel_vals.
+        all: iFrame; iRight; iFrame.
+        all: iRight; iFrame; iLeft; iFrame.
+  Qed.
+
+  (* TODO now reduce to IND-CCA *)
+
 
 End logrel.
